src/Local.v
@@ -1,0 +1,140 @@
+Require Import Relations.
+Require Import EquivDec.
+Require Import Equality.
+Require Import List.
+Require Import Bool.
+Require Import Lia.
+Require Import NArith.
+Require Import PArith.
+Require Import ZArith.
+Require Import FMapPositive.
+Require Import FSetPositive.
+Require Import EquivDec.
+Require Import Sorted.
+Require Import sflib.
+
+Require Import Basic.
+Require Import Order.
+Require Import Time.
+Require Import Lang.
+Require Import Promising.
+
+Set Implicit Arguments.
+
+
+Inductive rgT := {
+  rely_loc: Loc.t;
+  rely_val: Val.t;
+  guarantee: Loc.t -> Prop;
+}.
+
+Module RGs.
+  Definition t := list rgT.
+
+  Definition consistentT := forall (tid:Id.t) (eu:ExecUnit.t) (rgs:t), Prop.
+
+  Inductive consistent0 (c:consistentT) (tid:Id.t) (eu:ExecUnit.t): forall (rgs:t), Prop :=
+  | consistent_nil
+      eu'
+      (STEP: rtc (ExecUnit.state_step tid) eu eu')
+      (PROMISES: eu'.(ExecUnit.local).(Local.promises) = bot):
+      consistent0 c tid eu nil
+  | consistent_promise
+      eu' rg rgs
+      (STEP: ExecUnit.promise_step tid eu eu')
+      (GUARANTEE: rg.(guarantee) 0) (* TODO *)
+      (CONSISTENT: c tid eu' (rg::rgs)):
+      consistent0 c tid eu (rg::rgs)
+  | consistent_unlock
+      eu' rg rgs
+      (STEP: ExecUnit.promise_step tid eu eu') (* TODO: rg.(rely) *)
+      (CONSISTENT: c tid eu' rgs):
+      consistent0 c tid eu (rg::rgs)
+  .
+  Hint Constructors consistent0.
+
+  Inductive future (rgs:t) (eu1 eu2:ExecUnit.t): Prop :=
+  | future_intro
+      mem
+      (GUARANTEE: forall msg (MSG: In msg mem), Forall (fun rg => rg.(rely_loc) <> msg.(Msg.loc)) rgs)
+      (STATE: eu2.(ExecUnit.state) = eu1.(ExecUnit.state))
+      (LOCAL: eu2.(ExecUnit.local) = eu1.(ExecUnit.local))
+      (MEM: eu2.(ExecUnit.mem) = eu1.(ExecUnit.mem) ++ mem)
+  .
+  Hint Constructors future.
+
+  Inductive consistent (tid:Id.t) (eu:ExecUnit.t) (rgs:t): Prop :=
+  | consistent_intro
+      (CONSISTENT:
+         forall eu'
+           (GUARANTEE: future rgs eu eu'),
+           consistent0 consistent tid eu' rgs)
+  .
+  Hint Constructors consistent.
+
+  Inductive consistent_imm (tid:Id.t) (eu:ExecUnit.t) (rgs:t): Prop :=
+  | consistent_imm_intro
+      (CONSISTENT: consistent0 consistent_imm tid eu rgs)
+  .
+  Hint Constructors consistent_imm.
+
+  Inductive consistent_ex (tid:Id.t) (eu:ExecUnit.t) (rgs:t): Prop :=
+  | consistent_ex_intro
+      eu'
+      (GUARANTEE: future rgs eu eu')
+      (CONSISTENT: consistent0 consistent_ex tid eu' rgs)
+  .
+  Hint Constructors consistent_ex.
+End RGs.
+
+Module LMachine.
+  Inductive t := mk {
+    machine: Machine.t;
+    rgss: IdMap.t RGs.t;
+  }.
+
+  Definition init (p:program): t :=
+    mk
+      (Machine.init p)
+      (IdMap.map (fun _ => []) p).
+
+  Inductive consistent (m:t): Prop :=
+  | consistent_intro
+      rgs
+      (RGSS: IdMap.Forall2
+               (fun tid th rgs =>
+                  RGs.consistent
+                    tid
+                    (ExecUnit.mk th.(fst) th.(snd) m.(machine).(Machine.mem))
+                    rgs)
+               m.(machine).(Machine.tpool) m.(rgss))
+      (INTERLEAVING: IdMap.interleaving m.(rgss) rgs)
+      (GUARANTEE: StronglySorted (fun rg1 rg2 => ~ rg1.(guarantee) rg2.(rely_loc)) rgs)
+  .
+
+  Lemma init_consistent p:
+    consistent (init p).
+  Proof.
+    econs; ss.
+    - ii. rewrite ? IdMap.map_spec. destruct (IdMap.find id p); ss.
+      econs. s. econs. econs; eauto.
+      inv GUARANTEE. rewrite LOCAL. ss.
+    - econs 1. ii. revert FIND. rewrite IdMap.map_spec. destruct (IdMap.find id p); ss. congr.
+    - econs.
+  Qed.
+End LMachine.
+
+Lemma local_consistent_global_consistent_nil (* TODO: naming? *)
+        m
+        (RGSS: IdMap.Forall (fun _ l => l = []) m.(LMachine.rgss))
+        (CONSISTENT: LMachine.consistent m):
+  Machine.consistent ExecUnit.state_step m.(LMachine.machine).
+Proof.
+Admitted.
+
+Theorem local_consistent_global_consistent
+        m
+        (CONSISTENT: LMachine.consistent m):
+  Machine.consistent ExecUnit.step m.(LMachine.machine).
+Proof.
+Admitted.
